Some drafts for handling calls

Wavelet/Simulation/Call.lean
@@ -58,6 +58,8 @@ structure EncapFn Op χ [Arity Op] where
   ω : Nat
   fn : Fn Op χ ι ω
 
+def Fn.encap [Arity Op] (fn : Fn Op χ m n) : EncapFn Op χ := ⟨m, n, fn⟩
+
 structure EncapConfig Op χ V S [Arity Op] where
   ι : Nat
   ω : Nat
@@ -74,10 +76,17 @@ def EncapConfig.init {Op χ V S}
   EncapConfig Op χ V S :=
   ⟨ef.ι, ef.ω, Seq.Config.init ef.fn state args⟩
 
-/-- Augments the operator set with one custom function. -/
-inductive WithFns Op [Arity Op] {χ k} (fns : Vector (EncapFn Op χ) k)
+/-- Augments the operator set with a list of custom functions. -/
+inductive WithFns Op [Arity Op] {χ k} (fns : Vector (EncapFn Op χ) k) where
   | op (o : Op)
   | call (k : Fin k)
+
+inductive WithFn (Op : Type u) [Arity Op] {χ} (fn : EncapFn Op χ) : Type u where
+  | op (o : Op)
+  | call
+
+infixl:65 " w/ " => WithFns
+infixl:65 " w/ " => WithFn
 
 /-- States for the additional `k` functions. -/
 structure WithFns.State
@@ -87,8 +96,14 @@ structure WithFns.State
   (fns : Vector (EncapFn Op χ) k) where
   innerState : S
   fnStates : Vector (Option (EncapConfig Op χ V S)) k
-  inv_matching_io {i : Fin k} :
-    fnStates[i] = some ec → ec.ι = fns[i].ι ∧ ec.ω = fns[i].ω
+
+structure WithFn.State
+  Op χ V S
+  [Arity Op] [InterpConsts V]
+  [InterpOp Op V S] [DecidableEq χ]
+  (fn : EncapFn Op χ) where
+  innerState : S
+  config : Option (Seq.Config Op χ V S fn.ι fn.ω)
 
 instance
   [Arity Op]
@@ -97,6 +112,14 @@ instance
     | .call i => fns[i].ι
   ω | .op o => Arity.ω o
     | .call i => fns[i].ω
+
+instance
+  [Arity Op]
+  {fn : EncapFn Op χ} : Arity (WithFn Op fn) where
+  ι | .op o => Arity.ι o
+    | .call => fn.ι
+  ω | .op o => Arity.ω o
+    | .call => fn.ω
 
 inductive WithFns.Step
   [Arity Op] [InterpConsts V]
@@ -120,14 +143,6 @@ inductive WithFns.Step
         state with
         fnStates := state.fnStates.set i
           (some (EncapConfig.init fns[i] state.innerState inputVals))
-        -- Preserve that the invariant is preserved.
-        inv_matching_io := by
-          intros ec j hec
-          simp [Vector.getElem_set] at hec
-          split at hec <;> rename_i hj
-          · simp [EncapConfig.init] at hec
-            simp [← hec, hj]
-          · apply state.inv_matching_io hec
       }, none)
   | step_call_cont :
     state.fnStates[i] = some ec →
@@ -136,24 +151,52 @@ inductive WithFns.Step
       state
       ({ state with
         fnStates := state.fnStates.set i (some { ec with config := config' })
-        inv_matching_io := by sorry
       }, none)
   | step_call_ret :
-    (hec : state.fnStates[i] = some ec) →
+    state.fnStates[i] = some ec →
+    (_ : ec.ω = fns[i].ω) →
     ec.config.expr = .ret retVals →
     WithFns.Step fns (.call i) inputVals
       state
       (
-        { state with
-          fnStates := state.fnStates.set i none
-          inv_matching_io := by sorry
-        },
-        some (cast (by
-          congr 1
-          simp [Arity.ω]
-          apply (state.inv_matching_io hec).2
-        ) retVals),
+        { state with fnStates := state.fnStates.set i none },
+        some (cast (by congr) retVals),
       )
+
+inductive WithFn.Step
+  [Arity Op] [InterpConsts V]
+  [InterpOp Op V S] [DecidableEq χ]
+  (fn : EncapFn Op χ) :
+  (op : WithFn Op fn) →
+  Vector V (Arity.ι op) →
+  WithFn.State Op χ V S fn →
+  WithFn.State Op χ V S fn × Option (Vector V (Arity.ω op)) →
+  Prop where
+  | step_op :
+    InterpOp.Step o inputVals state.innerState (innerState', outputVals) →
+    WithFn.Step fn (.op o) inputVals state
+      ({ state with innerState := innerState' }, outputVals)
+  /-- Initialize call state without producing any outputs. -/
+  | step_call_init :
+    state.config = none →
+    WithFn.Step fn .call inputVals
+      state
+      ({
+        state with
+        config := some (Seq.Config.init fn.fn state.innerState inputVals)
+      }, none)
+  | step_call_cont :
+    state.config = some config →
+    Seq.Config.Step config config' →
+    WithFn.Step fn .call inputVals
+      state
+      ({ state with config := config' }, none)
+  | step_call_ret :
+    state.config = some config →
+    config.expr = .ret retVals →
+    WithFn.Step fn .call inputVals
+      state
+      ({ state with config := none }, some retVals)
 
 instance
   [Arity Op] [InterpConsts V]
@@ -162,4 +205,158 @@ instance
   : InterpOp (WithFns Op fns) V (WithFns.State Op χ V S fns) where
   Step := WithFns.Step fns
 
+instance
+  [Arity Op] [InterpConsts V]
+  [InterpOp Op V S] [DecidableEq χ]
+  (fn : EncapFn Op χ)
+  : InterpOp (WithFn Op fn) V (WithFn.State Op χ V S fn) where
+  Step := WithFn.Step fn
+
+example
+  [Arity Op] [InterpConsts V]
+  [InterpOp Op V S] [DecidableEq χ]
+  (fns : Vector (EncapFn Op χ) k)
+  (main : Fn (Op w/ fns) χ m n)
+  : Dataflow.Proc Op χ V m n := sorry
+
+example
+  [Arity Op] [InterpConsts V]
+  [InterpOp Op V S] [DecidableEq χ]
+  (fn : EncapFn Op χ)
+  (main : Fn (Op w/ fn) χ m n)
+  : Dataflow.Proc Op χ V m n := sorry
+
+example
+  [Arity Op] [InterpConsts V]
+  [InterpOp Op V S] [DecidableEq χ]
+  (fns₁ : Vector (EncapFn Op χ) k)
+  (fns₂ : Vector (EncapFn (Op w/ fns₁) χ) k)
+  (main : Fn (Op w/ fns₁ w/ fns₂) χ m n)
+  : Dataflow.Proc Op χ V m n := sorry
+
+example
+  [Arity Op] [InterpConsts V]
+  [InterpOp Op V S] [DecidableEq χ]
+  (fn₁ : EncapFn Op χ)
+  (fn₂ : EncapFn (Op w/ fn₁) χ)
+  (fn₃ : EncapFn (Op w/ fn₁ w/ fn₂) χ)
+  (main : Fn (Op w/ fn₁ w/ fn₂ w/ fn₃) χ m n)
+  : Dataflow.Proc Op χ V m n := sorry
+
+inductive Fns (χ : Type v) (V : Type w) (S : Type x) : Type u → Type (max (u + 1) v w x) where
+  | empty : Fns χ V S Op
+  | decl [Arity Op]
+    (rest : Fns χ V S Op)
+    (fn : EncapFn Op χ)
+    : Fns χ V S (Op w/ fn)
+
+section Example
+
+variable (Op χ V S : Type*)
+variable [Arity Op]
+
+def efn₁ : EncapFn Op χ := sorry
+def efn₂ : EncapFn (Op w/ (efn₁ Op χ)) χ := sorry
+def fns : Fns χ V S (Op w/ (efn₁ Op χ) w/ (efn₂ Op χ))
+  := .decl (.decl .empty (efn₁ Op χ)) (efn₂ Op χ)
+
+end Example
+
 end Wavelet.Seq
+
+namespace Wavelet.Dataflow
+
+open Op Seq
+
+structure EncapProc Op χ V [Arity Op] where
+  ι : Nat
+  ω : Nat
+  proc : Proc Op χ V ι ω
+
+structure EncapConfig Op χ V S [Arity Op] where
+  ι : Nat
+  ω : Nat
+  config : Dataflow.Config Op χ V S ι ω
+
+def EncapConfig.init {Op χ V S}
+  [Arity Op]
+  [InterpConsts V]
+  [InterpOp Op V S]
+  [DecidableEq χ]
+  (ef : EncapProc Op χ V)
+  (state : S)
+  (args : Vector V ef.ι) :
+  EncapConfig Op χ V S :=
+  ⟨ef.ι, ef.ω, Dataflow.Config.init ef.proc state args⟩
+
+/-- Augments the operator set with a vector of custom processes. -/
+inductive WithProcs Op [Arity Op] {χ V k} (procs : Vector (EncapProc Op χ V) k) where
+  | op (o : Op)
+  | proc (k : Fin k)
+
+infixl:65 " w/ " => WithProcs
+
+structure WithProcs.State
+  Op χ V S
+  [Arity Op] [InterpConsts V]
+  [InterpOp Op V S] [DecidableEq χ]
+  (fns : Vector (EncapProc Op χ V) k) where
+  innerState : S
+  procStates : Vector (Option (EncapConfig Op χ V S)) k
+
+instance
+  [Arity Op]
+  {procs : Vector (EncapProc Op χ V) k} : Arity (WithProcs Op procs) where
+  ι | .op o => Arity.ι o
+    | .proc i => procs[i].ι
+  ω | .op o => Arity.ω o
+    | .proc i => procs[i].ω
+
+inductive WithProcs.Step
+  [Arity Op] [InterpConsts V]
+  [InterpOp Op V S] [DecidableEq χ]
+  (procs : Vector (EncapProc Op χ V) k) :
+  (op : WithProcs Op procs) →
+  Vector V (Arity.ι op) →
+  WithProcs.State Op χ V S procs →
+  WithProcs.State Op χ V S procs × Option (Vector V (Arity.ω op)) →
+  Prop where
+  | step_op :
+    InterpOp.Step o inputVals state.innerState (innerState', outputVals) →
+    WithProcs.Step procs (.op o) inputVals state
+      ({ state with innerState := innerState' }, outputVals)
+  | step_proc_init :
+    state.procStates[i] = none →
+    WithProcs.Step procs (.proc i) inputVals
+      state
+      ({
+        state with
+        procStates := state.procStates.set i
+          (some (EncapConfig.init procs[i] state.innerState inputVals))
+      }, none)
+  | step_proc_cont :
+    state.procStates[i] = some pc →
+    Dataflow.Config.Step pc.config config' →
+    WithProcs.Step procs (.proc i) inputVals
+      state
+      ({ state with
+        procStates := state.procStates.set i (some { pc with config := config' })
+      }, none)
+  | step_proc_ret :
+    state.procStates[i] = some pc →
+    pc.config.chans.popVals procs[i].proc.outputs = some (retVals, chans') →
+    WithProcs.Step procs (.proc i) inputVals
+      state
+      (
+        { state with procStates := state.procStates.set i none },
+        some retVals,
+      )
+
+/-- Flatten the use of nested processes to get a single dataflow graph. -/
+def flatten
+  [Arity Op]
+  (procs : Vector (EncapProc Op χ V) k)
+  (main : Proc (Op w/ procs) χ V m n)
+  : Proc Op χ V m n := sorry
+
+end Wavelet.Dataflow
